\begin{exercise}{
    Prove or disprove the following semantic equivalence:
    \[ \wwhile{b}{S}\ \cong_{\text{\tiny SOS}}\ \wwhile{b}{(\wrepeat{S}{\neg b})}  \]
}
    We want to prove $\forall S \in \texttt{Stm}, b \in \texttt{Bexp}, s, s' \in \texttt{State}$
    \begin{gather*}
        \instr{\wwhile{b}{S}}{s} \Rightarrow^* s' \\
        \iff \\
        \instr{\wwhile{b}{(\wrepeat{S}{\neg b})}}{s} \Rightarrow^* s'
    \end{gather*}
    Let $S_r = \wrepeat{S}{\neg b}$ for brevity.
    We distinguish two cases:
    \begin{itemize}
        \item $\Bool{b} s = \text{ff}$
            \begin{align*}
                &\instr{\wwhile{b}{S}}{s}
                \\&\qquad\Rightarrow \instr{\wif{b}{(S;\wwhile{b}{S})}{skip}}{s}
                \\&\qquad\Rightarrow \instr{skip}{s}
                \\&\qquad\Rightarrow s
                \\
                &\instr{\wwhile{b}{S_r}}{s}
                \\&\qquad\Rightarrow \instr{\wif{b}{(S_r; \wwhile{b}{S_r})}{skip}}{s}
                \\&\qquad\Rightarrow \instr{skip}{s}
                \\&\qquad\Rightarrow s
            \end{align*}
        \item $\Bool{b} s = \text{tt}$
            \begin{align*}
                &\instr{\wwhile{b}{S}}{s}
                \\&\qquad\Rightarrow \instr{\wif{b}{(S;\wwhile{b}{S})}{skip}}{s}
                \\&\qquad\Rightarrow \instr{S;\wwhile{b}{S}}{s}
                \\
                &\instr{\wwhile{b}{S_r}}{s}
                \\&\qquad\Rightarrow \instr{\wif{b}{(S_r; \wwhile{b}{S_r})}{skip}}{s}
                \\&\qquad\Rightarrow \instr{S_r; \wwhile{b}{S_r}}{s}
            \end{align*}
            \begin{itemize}
                \item $(\implies)$ \vspace{0.2cm} \\
                    By induction on the length $k$ of the derivation $\instr{S;\wwhile{b}{S}}{s} \Rightarrow^k s'$
                    \begin{itemize}
                        \item base case $k=0$ \\
                            $\instr{S;\wwhile{b}{S}}{s} \Rightarrow^0 s'$ is trivially false, so the implication is true.
                        \item inductive case $k+1$ \vspace*{-0.3cm}
                            \[ \instr{S;\wwhile{b}{S}}{s} \Rightarrow^{k+1} s' \]
                            By the decomposition lemma $\exists k_1, k_2 \in \N, s'' \in \texttt{State} :$
                            \begin{gather*}
                                k_1 + k_2 = k + 1\qquad\qquad \instr{S}{s} \Rightarrow^{k_1} s'' \\
                                \instr{\wwhile{b}{S}}{s''} \Rightarrow^{k_2} s'
                            \end{gather*}
                            Then:
                            \begin{align*}
                                &\instr{S_r; \wwhile{b}{S_r}}{s}
                                \\&\qquad\Rightarrow \instr{(S;\wif{\neg b}{skip}{S_r}); \wwhile{b}{S_r}}{s}
                            \end{align*}
                            We proved in class $\forall S_1, S_2, S_3 \in \texttt{Stm}$ $(S_1;S_2);S_3\ \cong_{\text{\tiny SOS}}\ S_1;(S_2;S_3)$, so:
                            \begin{gather*}
                                \instr{(S;\wif{\neg b}{skip}{S_r}); \wwhile{b}{S_r}}{s} \Rightarrow^* s'
                                \\
                                \iff
                                \\
                                \instr{S;(\wif{\neg b}{skip}{S_r}; \wwhile{b}{S_r})}{s} \Rightarrow^* s'
                            \end{gather*}
                            And then, by the composition lemma:
                            \begin{align*}
                                &\instr{S;(\wif{\neg b}{skip}{S_r}; \wwhile{b}{S_r})}{s}
                                \\&\qquad\Rightarrow^* \instr{\wif{\neg b}{skip}{S_r}; \wwhile{b}{S_r}}{s''}
                            \end{align*}
                            We then distinguish two cases:
                            \begin{itemize}
                                \item $\Bool{b} s'' = \text{ff}$
                                    \begin{align*}
                                        &\instr{\wwhile{b}{S}}{s''}
                                        \\&\qquad\Rightarrow \instr{\wif{b}{(S; \wwhile{b}{S})}{skip}}{s''}
                                        \\&\qquad\Rightarrow \instr{skip}{s''}
                                        \\&\qquad\Rightarrow s''
                                        \\
                                        &\instr{\wif{\neg b}{skip}{S_r}; \wwhile{b}{S_r}}{s''}
                                        \\&\qquad\Rightarrow \instr{skip; \wwhile{b}{S_r}}{s''}
                                        \\&\qquad\Rightarrow \instr{\wwhile{b}{S_r}}{s''}
                                        \\&\qquad\Rightarrow \instr{\wif{b}{(S_r; \wwhile{b}{S_r})}{skip}}{s''}
                                        \\&\qquad\Rightarrow \instr{skip}{s''}
                                        \\&\qquad\Rightarrow s''
                                    \end{align*}
                                \item $\Bool{b} s'' = \text{tt}$
                                    \begin{align*}
                                        &\instr{\wwhile{b}{S}}{s''}
                                        \\&\qquad\Rightarrow \instr{\wif{b}{(S; \wwhile{b}{S})}{skip}}{s''}
                                        \\&\qquad\Rightarrow \instr{S; \wwhile{b}{S}}{s''}
                                        \\&\qquad\Rightarrow^{k_2 - 2} s'
                                        \\
                                        &\instr{\wif{\neg b}{skip}{S_r}; \wwhile{b}{S_r}}{s''}
                                        \\&\qquad\Rightarrow \instr{S_r; \wwhile{b}{S_r}}{s''}
                                    \end{align*}
                                    Since $\instr{S; \wwhile{b}{S}}{s''} \Rightarrow^{k_2 - 2} s'$ and $k_2 - 2 = k - k_1 - 1 \leq k$ the inductive hypothesis holds and thus $\instr{S_r; \wwhile{b}{S_r}}{s''} \Rightarrow^* s'$
                            \end{itemize}
                    \end{itemize}
                \item $(\impliedby)$ \vspace{0.2cm} \\
                    By induction on the length $k$ of the derivation $\instr{S_r; \wwhile{b}{S_r}}{s} \Rightarrow^k s'$
                    \begin{itemize}
                        \item base case $k=0$ \\
                            $\instr{S_r; \wwhile{b}{S_r}}{s} \Rightarrow^0 s'$ is trivially false, so the implication is true.
                        \item inductive case $k+1$ \vspace*{-0.3cm}
                        \[ \instr{S_r; \wwhile{b}{S_r}}{s} \Rightarrow^{k+1} s' \]
                        \begin{align*}
                            &\instr{S_r; \wwhile{b}{S_r}}{s}
                            \\&\qquad\Rightarrow \instr{(S; \wif{\neg b}{skip}{S_r}); \wwhile{b}{S_r}}{s}
                            \\&\qquad\Rightarrow^{k} s'
                        \end{align*}
                        \[ \iff \]
                        \begin{align*}
                            &\instr{S; (\wif{\neg b}{skip}{S_r}; \wwhile{b}{S_r})}{s}
                            \\&\qquad\Rightarrow^{k} s'
                        \end{align*}
                        By the decomposition lemma $\exists k_1, k_2 \in \N, s'' \in \texttt{State} :$
                        \begin{gather*}
                            k_1 + k_2 = k \qquad\qquad\qquad \instr{S}{s} \Rightarrow^{k_1} s'' \\
                            \instr{\wif{\neg b}{skip}{S_r}; \wwhile{b}{S_r}}{s''} \Rightarrow^{k_2} s'
                        \end{gather*}
                        Then, by the composition lemma:
                        \begin{align*}
                            &\instr{S; \wwhile{b}{S}}{s}
                            \\&\qquad\Rightarrow^* \instr{\wwhile{b}{S}}{s''}
                            \\&\qquad\Rightarrow \instr{\wif{b}{(S; \wwhile{b}{S})}{skip}}{s''}
                        \end{align*}
                        We distinguish two cases:
                        \begin{itemize}
                            \item $\Bool{b} s'' = \text{ff}$
                                \begin{align*}
                                    &\instr{\wif{\neg b}{skip}{S_r}; \wwhile{b}{S_r}}{s''}
                                    \\&\qquad\Rightarrow \instr{skip; \wwhile{b}{S_r}}{s''}
                                    \\&\qquad\Rightarrow \instr{\wwhile{b}{S_r}}{s''}
                                    \\&\qquad\Rightarrow \instr{\wif{b}{(S_r; \wwhile{b}{S_r})}{skip}}{s''}
                                    \\&\qquad\Rightarrow \instr{skip}{s''}
                                    \\&\qquad\Rightarrow s''
                                    \\
                                    &\instr{\wif{b}{(S; \wwhile{b}{S})}{skip}}{s''}
                                    \\&\qquad\Rightarrow \instr{skip}{s''}
                                    \\&\qquad\Rightarrow s''
                                \end{align*}
                            \item $\Bool{b} s'' = \text{tt}$
                                \begin{align*}
                                    &\instr{\wif{\neg b}{skip}{S_r}; \wwhile{b}{S_r}}{s''}
                                    \\&\qquad\Rightarrow \instr{S_r; \wwhile{b}{S_r}}{s''}
                                    \\&\qquad\Rightarrow^{k_2 - 1} s'
                                    \\
                                    &\instr{\wif{b}{(S; \wwhile{b}{S})}{skip}}{s''}
                                    \\&\qquad\Rightarrow \instr{S; \wwhile{b}{S}}{s''}
                                \end{align*}
                                Since $\instr{S_r; \wwhile{b}{S_r}}{s''} \Rightarrow^{k_2 - 1} s'$ and $k_2 - 1 = k - k_1 - 1 \leq k$ the inductive hypothesis holds and thus $\instr{S; \wwhile{b}{S}}{s''} \Rightarrow^* s'$
                        \end{itemize}
                    \end{itemize}
            \end{itemize}
    \end{itemize}
\end{exercise}
