\begin{exercise}{
    Prove or disprove the following semantic equivalence:
    \[ \wwhile{b}{S} \cong_{\text{\tiny SOS}} \wwhile{b}{(\wwhile{b}{S})}  \]\vspace*{-0.6cm}
}
    We want to prove $\forall S \in \texttt{Stm}, b \in \texttt{Bexp}, s, s' \in \texttt{State}$
    \begin{gather*}
        \instr{\wwhile{b}{S}}{s} \Rightarrow^* s' \\
        \iff \\
        \instr{\wwhile{b}{(\wwhile{b}{S})}}{s} \Rightarrow^* s'
    \end{gather*}
    We distinguish two cases:
    \begin{itemize}
        \item $\Bool{b} s = \text{ff}$
            \begin{align*}
                &\instr{\wwhile{b}{S}}{s}
                \\&\qquad\Rightarrow \instr{\wif{b}{(S; \wwhile{b}{S})}{skip}}{s}
                \\&\qquad\Rightarrow \instr{skip}{s}
                \\&\qquad\Rightarrow s
                \\
                &\instr{\wwhile{b}{(\wwhile{b}{S})}}{s}
                \\&\qquad\Rightarrow \instr{\wif{b}{(\wwhile{b}{S}; \wwhile{b}{(\wwhile{b}{S})})}{skip}}{s}
                \\&\qquad\Rightarrow \instr{skip}{s}
                \\&\qquad\Rightarrow s
            \end{align*}
        \item $\Bool{b} s = \text{tt}$
            \begin{align*}
                &\instr{\wwhile{b}{(\wwhile{b}{S})}}{s}
                \\&\qquad\Rightarrow \instr{\wif{b}{(\wwhile{b}{S}; \wwhile{b}{(\wwhile{b}{S})})}{skip}}{s}
                \\&\qquad\Rightarrow \instr{\wwhile{b}{S}; \wwhile{b}{(\wwhile{b}{S})}}{s}
            \end{align*}
            \begin{itemize}
                \item $(\implies)$
                    \[ \instr{\wwhile{b}{S}}{s} \Rightarrow^* s' \]
                    By the termination lemma $\Bool{b} s' = \text{ff}$. Then, by the composition lemma:
                    \begin{align*}
                        &\instr{\wwhile{b}{S}; \wwhile{b}{(\wwhile{b}{S})}}{s}
                        \\&\qquad\Rightarrow^* \instr{\wwhile{b}{(\wwhile{b}{S})}}{s'}
                        \\&\qquad\Rightarrow \instr{\wif{b}{(\wwhile{b}{S}; \wwhile{b}{(\wwhile{b}{S})})}{skip}}{s'}
                        \\&\qquad\Rightarrow \instr{skip}{s'}
                        \\&\qquad\Rightarrow s'
                    \end{align*}
                \item $(\impliedby)$
                    \[ \instr{\wwhile{b}{S}; \wwhile{b}{(\wwhile{b}{S})}}{s} \Rightarrow^* s' \]
                    By the decomposition lemma:
                    \[
                        \instr{\wwhile{b}{S}}{s} \Rightarrow^* s''
                        \qquad
                        \instr{\wwhile{b}{(\wwhile{b}{S})}}{s''} \Rightarrow^* s'
                    \]
                    By the termination lemma $\Bool{b} s'' = \text{ff}$. Thus:
                    \begin{align*}
                        &\instr{\wwhile{b}{(\wwhile{b}{S})}}{s''}
                        \\&\qquad\Rightarrow \instr{\wif{b}{(\wwhile{b}{S}; \wwhile{b}{(\wwhile{b}{S})})}{skip}}{s''}
                        \\&\qquad\Rightarrow \instr{skip}{s''}
                        \\&\qquad\Rightarrow s'' = s'
                    \end{align*}
                    Thus $\instr{\wwhile{b}{S}}{s} \Rightarrow^* s'' = s'$
            \end{itemize}
    \end{itemize}
\end{exercise}
