\begin{exercise}{
    Prove or disprove the following semantic equivalence:
    \[ \wwhile{b}{S}\ \cong_{\text{\tiny SOS}}\ \wwhile{b}{(S;\wif{b}{S}{skip})} \]
}
    We want to prove $\forall S \in \texttt{Stm}, b \in \texttt{Bexp}, s, s' \in \texttt{State}$
    \begin{gather*}
        \instr{\wwhile{b}{S}}{s} \Rightarrow^* s' \\
        \iff \\
        \instr{\wwhile{b}{(S;\wif{b}{S}{skip})}}{s} \Rightarrow^* s'
    \end{gather*}
    Let $S_s = \wwhile{b}{(S;\wif{b}{S}{skip})}$ for brevity.
    \begin{itemize}
        \item $(\implies)$ \\
            By induction on the length $k$ of the derivation $\instr{\wwhile{b}{S}}{s} \Rightarrow^k s'$
            \begin{itemize}
                \item base case $k=0$ \\
                    $\instr{\wwhile{b}{S}}{s} \Rightarrow^0 s'$ is trivially false, so the implication is true.
                \item inductive case $k+1$
                    \[ \instr{\wwhile{b}{S}}{s} \Rightarrow^{k+1} s' \]
                    We distinguish two cases:
                    \begin{itemize}
                        \item $\Bool{b} s = \text{ff}$
                            \begin{align*}
                                &\instr{\wwhile{b}{S}}{s}
                                \\&\qquad\Rightarrow \instr{\wif{b}{(S; \wwhile{b}{S})}{skip}}{s}
                                \\&\qquad\Rightarrow \instr{skip}{s}
                                \\&\qquad\Rightarrow s
                                \\
                                &\instr{S_s}{s}
                                \\&\qquad\Rightarrow \instr{\wif{b}{((S;\wif{b}{S}{skip});S_s)}{skip}}{s}
                                \\&\qquad\Rightarrow \instr{skip}{s}
                                \\&\qquad\Rightarrow s
                            \end{align*}
                        \item $\Bool{b} s = \text{tt}$
                            \begin{align*}
                                &\instr{\wwhile{b}{S}}{s}
                                \\&\qquad\Rightarrow \instr{\wif{b}{(S; \wwhile{b}{S})}{skip}}{s}
                                \\&\qquad\Rightarrow \instr{S; \wwhile{b}{S}}{s}
                                \\&\qquad\Rightarrow^{k-1} s'
                            \end{align*}
                            By the decomposition lemma $\exists k_1, k_2 \in \mathbb{N}, s'' \in \texttt{State} :$
                            \begin{gather*}
                                k_1 + k_2 = k - 1 \qquad\qquad\qquad \instr{S}{s} \Rightarrow^{k_1} s'' \\
                                \instr{\wwhile{b}{S}}{s''} \Rightarrow^{k_2} s'
                            \end{gather*}
                            Then:
                            \begin{align*}
                                &\instr{S_s}{s}
                                \\&\qquad\Rightarrow \instr{\wif{b}{((S;\wif{b}{S}{skip});S_s)}{skip}}{s}
                                \\&\qquad\Rightarrow \instr{(S;\wif{b}{S}{skip});S_s}{s}
                            \end{align*}
                            We proved in class $\forall S_1, S_2, S_3 \in \texttt{Stm}$ $(S_1;S_2);S_3\ \cong_{\text{\tiny SOS}}\ S_1;(S_2;S_3)$, so:
                            \begin{gather*}
                                \instr{(S;\wif{b}{S}{skip});S_s}{s} \Rightarrow^* s'
                                \\
                                \iff
                                \\
                                \instr{S;(\wif{b}{S}{skip};S_s)}{s} \Rightarrow^* s'
                            \end{gather*}
                            By the composition lemma:
                            \[
                                \instr{S;(\wif{b}{S}{skip};S_s)}{s}
                                \Rightarrow^*
                                \instr{\wif{b}{S}{skip};S_s}{s''}
                            \]
                            We distinguish two cases:
                            \begin{itemize}
                                \item $\Bool{b} s'' = \text{ff}$
                                    \begin{align*}
                                        &\instr{\wwhile{b}{S}}{s''}
                                        \\&\qquad\Rightarrow \instr{\wif{b}{(S; \wwhile{b}{S})}{skip}}{s''}
                                        \\&\qquad\Rightarrow \instr{skip}{s''}
                                        \\&\qquad\Rightarrow s''
                                        \\
                                        &\instr{\wif{b}{S}{skip};S_s}{s''}
                                        \\&\qquad\Rightarrow \instr{skip;S_s}{s''}
                                        \\&\qquad\Rightarrow \instr{S_s}{s''}
                                        \\&\qquad\Rightarrow \instr{\wif{b}{((S;\wif{b}{S}{skip});S_s)}{skip}}{s''}
                                        \\&\qquad\Rightarrow \instr{skip}{s''}
                                        \\&\qquad\Rightarrow s''
                                    \end{align*}
                                \item $\Bool{b} s'' = \text{tt}$
                                    \begin{align*}
                                        &\instr{\wwhile{b}{S}}{s''}
                                        \\&\qquad\Rightarrow \instr{\wif{b}{(S; \wwhile{b}{S})}{skip}}{s''}
                                        \\&\qquad\Rightarrow \instr{S; \wwhile{b}{S}}{s''}
                                        \\&\qquad\Rightarrow^{k_2 - 2} s'
                                    \end{align*}
                                    By the decomposition lemma $\exists k_3, k_4 \in \mathbb{N}, s''' \in \texttt{State} :$
                                    \begin{gather*}
                                        k_3 + k_4 = k_2 - 2 \qquad\qquad\qquad \instr{S}{s''} \Rightarrow^{k_3} s''' \\
                                        \instr{\wwhile{b}{S}}{s'''} \Rightarrow^{k_4} s'
                                    \end{gather*}
                                    Thus by the composition lemma:
                                    \[
                                        \instr{\wif{b}{S}{skip};S_s}{s''}
                                        \Rightarrow \instr{S;S_s}{s''}
                                        \Rightarrow^* \instr{S_s}{s'''}
                                    \]
                                    Since $\instr{\wwhile{b}{S}}{s'''} \Rightarrow^{k_4} s'$ and $k_4 = k - k_1 - k_3 - 3 \leq k$ the inductive hypothesis holds and thus $\instr{S_s}{s'''} \Rightarrow^* s'$
                            \end{itemize}
                    \end{itemize}
            \end{itemize}
        \item $(\impliedby)$ \\
            By induction on the length $k$ of the derivation $\instr{S_s}{s} \Rightarrow^k s'$
            \begin{itemize}
                \item base case $k=0$ \\
                    $\instr{S_s}{s} \Rightarrow^0 s'$ is trivially false, so the implication is true.
                \item inductive case $k+1$
                    \[ \instr{S_s}{s} \Rightarrow^{k+1} s' \]
                    We distinguish two cases:
                    \begin{itemize}
                        \item $\Bool{b} s = \text{ff}$
                            \begin{align*}
                                &\instr{S_s}{s}
                                \\&\qquad\Rightarrow \instr{\wif{b}{((S;\wif{b}{S}{skip});S_s)}{skip}}{s}
                                \\&\qquad\Rightarrow \instr{skip}{s}
                                \\&\qquad\Rightarrow s
                                \\
                                &\instr{\wwhile{b}{S}}{s}
                                \\&\qquad\Rightarrow \instr{\wif{b}{(S; \wwhile{b}{S})}{skip}}{s}
                                \\&\qquad\Rightarrow \instr{skip}{s}
                                \\&\qquad\Rightarrow s
                            \end{align*}
                        \item $\Bool{b} s = \text{tt}$
                            \begin{align*}
                                &\instr{S_s}{s}
                                \\&\qquad\Rightarrow \instr{\wif{b}{((S;\wif{b}{S}{skip});S_s)}{skip}}{s}
                                \\&\qquad\Rightarrow \instr{(S;\wif{b}{S}{skip});S_s}{s}
                                \\&\qquad\Rightarrow^{k - 1} s'
                            \end{align*}
                            By the decomposition lemma $\exists k_1, k_2 \in \mathbb{N}, s'' \in \texttt{State} :$
                            \begin{gather*}
                                k_1 + k_2 = k + 1 \qquad\qquad\qquad \instr{S;\wif{b}{S}{skip}}{s} \Rightarrow^{k_1} s'' \\
                                \instr{S_s}{s''} \Rightarrow^{k_2} s'
                            \end{gather*}
                            Then, by the decomposition lemma $\exists s''' :$
                            \begin{gather*}
                                \instr{S}{s} \Rightarrow^* s''' \\
                                \instr{\wif{b}{S}{skip}}{s'''} \Rightarrow^* s''
                            \end{gather*}
                            Then, by the composition lemma:
                            \begin{align*}
                                &\instr{\wwhile{b}{S}}{s}
                                \\&\qquad\Rightarrow \instr{\wif{b}{(S; \wwhile{b}{S})}{skip}}{s}
                                \\&\qquad\Rightarrow \instr{S; \wwhile{b}{S}}{s}
                                \\&\qquad\Rightarrow^* \instr{\wwhile{b}{S}}{s'''}
                                \\&\qquad\Rightarrow \instr{\wif{b}{(S; \wwhile{b}{S})}{skip}}{s'''}
                            \end{align*}
                            We distinguish two cases:
                            \begin{itemize}
                                \item $\Bool{b} s''' = \text{ff}$
                                    \begin{align*}
                                        &\instr{\wif{b}{S}{skip}}{s'''}
                                        \\&\qquad\Rightarrow \instr{skip}{s'''}
                                        \\&\qquad\Rightarrow s''' = s''
                                        \\
                                        &\instr{S_s}{s'''}
                                        \\&\qquad\Rightarrow \instr{\wif{b}{((S;\wif{b}{S}{skip});S_s)}{skip}}{s'''}
                                        \\&\qquad\Rightarrow \instr{skip}{s'''}
                                        \\&\qquad\Rightarrow s'''
                                        \\
                                        &\instr{\wif{b}{(S; \wwhile{b}{S})}{skip}}{s'''}
                                        \\&\qquad\Rightarrow \instr{skip}{s'''}
                                        \\&\qquad\Rightarrow s'''
                                    \end{align*}
                                \item $\Bool{b} s''' = \text{tt}$
                                    \begin{align*}
                                        &\instr{\wif{b}{S}{skip}}{s'''}
                                        \\&\qquad\Rightarrow \instr{S}{s'''}
                                        \\&\qquad\Rightarrow^* s''
                                    \end{align*}
                                    Thus, by the composition lemma:
                                    \begin{align*}
                                        &\instr{\wif{b}{(S; \wwhile{b}{S})}{skip}}{s'''}
                                        \\&\qquad\Rightarrow \instr{S; \wwhile{b}{S}}{s'''}
                                        \\&\qquad\Rightarrow^* \instr{\wwhile{b}{S}}{s''}
                                    \end{align*}
                                    Since $\instr{S_s}{s''} \Rightarrow^{k_2} s'$ and $k_2 = k - k_1 - 1 \leq k$ the inductive hypothesis holds and thus $\instr{\wwhile{b}{S}}{s''} \Rightarrow^* s'$
                            \end{itemize}
                    \end{itemize}
            \end{itemize}
    \end{itemize}
\end{exercise}
