\begin{exercise}{
    Prove that if $\Sds{\wwhile{b}{S}} s = s'$ then $\Bool{b} s' = \text{ff}$
}
    Recall that $\Sds{\wwhile{b}{S}} = \FIX F$ where $F\ g= \cond{\Bool{b}}{g \circ \Sds{S}}{\id}$ is a continuous function. \\
    Then consider the following function:
    \[
        d\ s = \begin{cases}
            \undef &\quad \text{if } (\FIX F)\ s = s' \neq \undef, \Bool{b} s' = \text{tt} \\
            (\FIX F)\ s &\quad \text{otherwise}
        \end{cases}
    \]
    We prove that $F d \sqsubseteq d$, that is:
    \[ \forall s, s' \in \texttt{State}\ (F\ d) s = s' \implies d\ s = s' \]
    We distinguish two cases:
    \begin{itemize}
        \item $\Bool{b} s = \text{ff}$
            \[ (F\ d) s = \cond{\Bool{b}}{d \circ \Sds{S}}{\id} = \id s = s = s' \]
            Thus $\Bool{b} s' = \Bool{b} s = \text{ff}$
            \[ (\FIX F)\ s = F(\FIX F)\ s = \cond{\Bool{b}}{\FIX F \circ \Sds{S}}{\id} = \id s = s = s' \]
            Since $(\FIX F)\ s = s \neq \undef$ and $\Bool{b} s \neq \text{tt}$ we have $d\ s = (\FIX F)\ s = s$
        \item $\Bool{b} s = \text{tt}$
            \[ (F\ d) s = \cond{\Bool{b}}{d \circ \Sds{S}}{\id} = (d \circ \Sds{S})\ s \]
            We then distinguish two cases:
            \begin{itemize}
                \item $\Sds{S}\ s = \undef$, thus $(d \circ \Sds{S})\ s = \undef$, the premise is false and thus the implication is true;
                \item $\Sds{S}\ s = s'' \neq \undef$, thus $(d \circ \Sds{S})\ s = d\ s''$
                    \begin{align*}
                        (\FIX F)\ s &= F(\FIX F)\ s = \cond{\Bool{b}}{\FIX F \circ \Sds{S}}{\id} \\
                        &= (\FIX F \circ \Sds{S})\ s = (\FIX F)\ s''
                    \end{align*}
                    We distinguish two cases:
                    \begin{itemize}
                        \item $(\FIX F)\ s = (\FIX F)\ s'' = s''' \neq \undef, \Bool{b} s''' = \text{tt}$, then $d\ s'' = \undef = d\ s$
                        \item otherwise, $d\ s'' = (\FIX F)\ s'' = (\FIX F)\ s = d\ s$
                    \end{itemize}
            \end{itemize}
    \end{itemize}
    Thus by the fixpoint induction lemma we have $\FIX F \sqsubseteq d$. which means that:
    \[ \forall s, s' \in \texttt{State}\ (\FIX F)\ s = s' \implies d\ s = s' \]
    Assume by contradiction that $\exists s, s' \in \texttt{State} : (\FIX F)\ s = s', \Bool{b} s' = \text{tt} $. Then $d\ s = \undef \neq s'$, which means $\FIX F \not\sqsubseteq d$, and that's a contradiction. Thus $(\FIX F)\ s = s' \implies \Bool{b} s' = \text{ff}$
\end{exercise}
