\begin{exercise}{
    Prove or disprove the following semantic equivalence:
    \[ \wwhile{b}{S} \DScong (\wwhile{b}{S});(\wwhile{b}{S}) \]
}
    We want to prove $\Sds{\wwhile{b}{S}} = \Sds{(\wwhile{b}{S});(\wwhile{b}{S})}$, that is $\FIX F = \FIX F \circ \FIX F$ where $F\ g = \cond{\Bool{b}}{g \circ \Sds{S}}{\id}$
    \begin{itemize}
        \item $\FIX F \sqsubseteq \FIX F \circ \FIX F$
            \[ \forall s, s' \in \State\ (\FIX F)\ s = s' \implies (\FIX F \circ \FIX F)\ s = s' \]
            By the termination lemma (see exercise 7) we have $\Bool{b} s' = \False$.
            \begin{align*}
                (\FIX F \circ \FIX F)\ s &= (\FIX F)\ s' = F(\FIX F)\ s = \\
                &= \cond{\Bool{b}}{\FIX F \circ \Sds{S}}{\id} s' = \\
                &= \id s' = s'
            \end{align*}
        \item $\FIX F \sqsupseteq \FIX F \circ \FIX F$
            \[ \forall s, s' \in \State\ (\FIX F \circ \FIX F)\ s = s' \implies (\FIX F)\ s = s' \]
            By the definition of function composition:
            \[
                (\FIX F \circ \FIX F)\ s = \begin{cases}
                    (\FIX F \circ \FIX F)\ s &\quad \text{if } (\FIX F)\ s \neq \undef, \\
                        &\quad\quad (\FIX F \circ \FIX F)\ s \neq \undef \\
                    \undef &\quad \text{otherwise}
                \end{cases}
            \]
            Since $(\FIX F \circ \FIX F)\ s = s' \neq \undef$ we must have $(\FIX F)\ s = s'' \neq \undef$. Thus, by the termination lemma $\Bool{b} s'' = \False$, and so:
            \begin{align*}
                (\FIX F \circ \FIX F)\ s &= (\FIX F)\ s'' = F(\FIX F)\ s'' = \\
                &= \cond{\Bool{b}}{\FIX F \circ \Sds{S}}{\id} s'' = \\
                &= \id s'' = s'' = s'
            \end{align*}
            Thus $(\FIX F)\ s = s'' = s'$
    \end{itemize}
\end{exercise}
